ExprEval/BoolStepLemmas.lean
@@ -1,0 +1,52 @@
+import ExprEval.Expr
+import ExprEval.Boolean
+
+theorem boolstep_preserves_eval_bool (e e': BoolExpr V):
+  BoolStep val e e' -> eval_bool val e = eval_bool val e' := by
+  intro h
+  induction h with
+  | notIsBoolNot b => simp [eval_bool]
+  | andLeftTrue e => simp [eval_bool]
+  | orLeftFalse e => simp [eval_bool]
+  | andLeftShortCircuit e => simp [eval_bool]
+  | orLeftShortCircuit e => simp [eval_bool]
+  | lessConstConstTrue n1 n2 h =>
+    simp [eval_bool]
+    simp [eval]
+    exact h
+  | lessConstConstFalse n1 n2 h =>
+    simp [eval_bool]
+    simp [eval]
+    exact h
+  | eqConstConstTrue n1 n2 h =>
+    simp [eval_bool]
+    simp [eval]
+    exact h
+  | eqConstConstFalse n1 n2 h =>
+    simp [eval_bool]
+    simp [eval]
+    simp [bne_iff_ne] at h
+    exact h
+  | lessArStepLeft e₁ e₁' e₂ arstep
+  | eqArStepLeft e₁ e₁' e₂ arstep
+  | lessArStepRight e₁ e₂ e₂' arstep
+  | eqArStepRight e₁ e₂ e₂' arstep =>
+    simp [eval_bool]
+    have h' := arstep_preserve_eval _ _ _ arstep
+    rw [h']
+  | orStepLeft e₁ e₁' e₂ step ihn
+  | andStepLeft e₁ e₁' e₂ step ihn =>
+    simp [eval_bool]
+    rw [ihn]
+  | notStep e e' step ihn =>
+    simp[eval_bool]
+    rw [ihn]
+
+theorem boolstepstar_preserves_eval_bool (e e': BoolExpr V):
+  BoolStepStar V val e e' -> eval_bool val e = eval_bool val e' := by
+  intro h
+  induction h with
+  | refl => rfl
+  | trans _ _ _ h_step _ ihn =>
+    rw [<- ihn]
+    exact boolstep_preserves_eval_bool _ _ h_step
